fix: calling trait requirement functions which have local trait requirements

case_studies/tests/src/trait_deps.rs
@@ -1,4 +1,78 @@
 
+// WIP: handle obligations on associated types
+/*
+mod bla {
+    trait Bupsed {
+
+    }
+
+    #[rr::exists("bb" : "{xt_of BB}")]
+    trait Bar {
+        type BB: Bupsed;
+    }
+    
+    trait Foo {
+        type FB: Bar;
+
+        // this specification should maybe depend on Bar
+        // i.e. I need the trait attributes of Bar
+        //
+        // For now, this is also problematic because we do not add FB's env here.
+        #[rr::verify]
+        #[rr::returns("{Self::FB::bb}")]
+        fn bla() -> <<Self as Foo>::FB as Bar>::BB;
+    }
+    // Should the attrs record be allowed to depend on the attrs record of Bar?
+    // I don't think so. This is different from a normal trait context assumption, so it shouldn't
+    // depend on that. This is an obligation at the impl site, not a requirement.
+    //
+    // Can the attrs record depend on the associated type? I hope not.
+    //
+    // Can the spec record depend? Yeah, it should be allowed to depend on the obligation assoc types, because the type signature of the functions may depend on that.
+    // not attrs.
+
+
+    // Issue here: I see the obligation as a Self requirement and thus do not add it to the env.
+    // Probably this shouldn't be just skipped. 
+    // how do I handle the trait's own associated types? I guess they cannot be normalized.
+
+    impl Bupsed for bool {
+
+    }
+
+    #[rr::instantiate("bb" := "true")]
+    impl Bar for u32 {
+        type BB = bool;
+    }
+
+    impl Foo for i32 {
+        type FB = u32;
+    
+        #[rr::default_spec]
+        fn bla() -> bool {
+            true
+        }
+    }
+
+    impl<T: Bar> Foo for (u32, T) {
+        type FB = T;
+
+        #[rr::default_spec]
+        fn bla() -> <T as Bar>::BB {
+            unimplemented!();
+        }
+    }
+
+    #[rr::verify]
+    fn foo<T>() 
+        where T: Foo<FB = u32>,
+              T::FB: Bar<BB = bool>
+    {
+
+    }
+}
+*/
+
 // I want an example where I need to distinguish different sources of trait requirements.
 mod dep {
     trait Bar {
